Classs updates

website/code/Fibonacci.dfy
@@ -1,12 +1,29 @@
+function fib(n:nat) : nat {
+   match n 
+      case 0 => 0 
+      case 1 => 1
+      case _ => fib (n-1) + fib (n-2)
+}
+
 method ComputeFib(n: nat) returns (b: nat)
+   requires true 
+   ensures b == fib(n)
 {
    if n == 0 { return 0; }
    var i: int := 1;
    var a := 0;
        b := 1;
    while i < n
+      invariant i <= n
+      invariant b == fib(i)
+      invariant a == fib(i-1)
    {
       a, b := b, a + b;
       i := i + 1;
    }
+   // b == fib(i)
+   // a == fib(i-1)
+   // !(i<n)
+   // ------
+   // b == fib(n)
 }
