website/code/HoareLogicAssertions.dfy
@@ -1,0 +1,611 @@
+/** Hoare Triples and Dafny */
+
+/** A _Hoare triple_ is a claim about the state before and
+    after executing a statement.  The standard notation is
+
+      {P} s {Q}
+
+    meaning:
+
+      - If statement s begins execution in a state satisfying assertion P,
+      - and if s eventually terminates in some final state,
+      - then that final state will satisfy the assertion Q.
+
+    Assertion P is called the _precondition_ of the triple, and Q is
+    the _postcondition_.
+
+    For example,
+
+    - {x == 0} x := x + 1 {x == 1} is a valid Hoare triple,
+      stating that the statement x := x + 1 would transform a state in
+      which x == 0 to a state in which x == 1.
+
+    - forall m, {x == m} x := x + 1 {x == m + 1}, is a
+      _proposition_ stating that the Hoare triple {x == m} x := x +
+      m {x == m + 1} is valid for any choice of m.  Note that m
+      in the two assertions and the command in the middle is a
+      reference to the _Dafny_ variable m, which is bound outside the
+      Hoare triple. */
+
+/* ################################################################# */
+/** * Proof Rules */
+
+/** The goal of Hoare logic is to provide a _compositional_
+    method for proving the validity of specific Hoare triples.  That
+    is, we want the structure of a program's correctness proof to
+    mirror the structure of the program itself.  To this end, in the
+    sections below, we'll introduce a rule for reasoning about each of
+    the different syntactic forms of statements in Dafny -- one for
+    assignment, one for sequencing, one for conditionals, etc. -- plus
+    a couple of "structural" rules for gluing things together.  We
+    will then be able to prove programs correct using these proof
+    rules. */
+
+/* ================================================================= */
+/** ** Empty statement blocks 
+
+/** Since empty statement blocks don't change the state, they preserve any
+    assertion [P]:
+
+      --------------------  (hoare_skip)
+         { P } {} { P }
+*/
+
+/* ================================================================= */
+/** ** Sequencing 
+
+/** If statement s1 takes any state where P holds to a state where
+    Q holds, and if s2 takes any state where Q holds to one
+    where R holds, then doing s1 followed by s2 will take any
+    state where P holds to one where R holds:
+
+        { P } s1 { Q }
+        { Q } s2 { R }
+       ----------------------  (hoare_seq)
+       { P } s1;s2 { R }
+*/
+
+/* ================================================================= */
+/** ** Assignment */
+
+/** The rule for assignment is the most fundamental of the Hoare
+    logic proof rules.  Here's how it works.
+
+    Consider this incomplete Hoare triple:
+
+       { ??? }}  x := y  { x == 1 }
+
+    We want to assign y to x and finish in a state where x is 1.
+    What could the precondition be?
+
+    One possibility is y == 1, because if y is already 1 then
+    assigning it to x causes x to be 1.  That leads to a valid
+    Hoare triple:
+
+       { y == 1 }  x := y  { x == 1 }
+
+    It may seem as though coming up with that precondition must have
+    taken some clever thought.  But there is a mechanical way we could
+    have done it: if we take the postcondition x == 1 and in it
+    replace x with y---that is, replace the left-hand side of the
+    assignment statement with the right-hand side---we get the
+    precondition, y = 1. 
+
+    That same idea works in more complicated cases.  For
+    example:
+
+       { ??? }  x := x + y  { x == 1 }
+
+    If we replace the x in x == 1 with x + y, we get x + y == 1.
+    That again leads to a valid Hoare triple:
+
+       { x + y == 1 }  x := x + y  { x == 1 }
+
+    Why does this technique work?  The postcondition identifies some
+    property P that we want to hold of the variable x being
+    assigned.  In this case, P is "equals 1".  To complete the
+    triple and make it valid, we need to identify a precondition that
+    guarantees that property will hold of x.  Such a precondition
+    must ensure that the same property holds of _whatever is being
+    assigned to_ x.  So, in the example, we need "equals 1" to
+    hold of x + y.  That's exactly what the technique guarantees. 
+
+    In general, the postcondition could be some arbitrary assertion
+    Q, and the right-hand side of the assignment could be some
+    arbitrary arithmetic expression a:
+
+       { ??? }  x := a  { Q }
+
+    The precondition would then be Q, but with any occurrences of
+    x in it replaced by a.
+
+    Let's introduce a notation for this idea of replacing occurrences:
+    Define Q[x := a] to mean "Q where a is substituted in
+    place of x".
+
+    This yields the Hoare logic rule for assignment:
+
+      { Q[x := a] }  x := a  { Q }
+
+    One way of reading this rule is: If you want statement x := a
+    to terminate in a state that satisfies assertion Q, then it
+    suffices to start in a state that also satisfies Q, except
+    where a is substituted for every occurrence of x. *)
+
+    To many people, this rule seems "backwards" at first, because
+    it proceeds from the postcondition to the precondition.  Actually
+    it makes good sense to go in this direction: the postcondition is
+    often what is more important, because it characterizes what we
+    can assume afer running the code.
+
+    Nonetheless, it's also possible to formulate a "forward" assignment
+    rule. 
+*/
+
+/** Here are some valid instances of the assignment rule:
+
+      { (x <= 5) [x := x + 1] }   (that is, X + 1 <= 5)
+        x := x + 1
+      { x <= 5 }
+
+      { (x == 3) [x := 3] }        (that is, 3 = 3)
+        x := 3
+      { x = 3 }
+
+      { (0 <= x && x <= 5) [X := 3]  (that is, 0 <= 3 /\ 3 <= 5)
+        x := 3
+      { 0 <= x && x <= 5 }}
+*/
+
+/* ================================================================= */
+/** ** Consequence 
+
+    Sometimes the preconditions and postconditions we get from the
+    Hoare rules won't quite be the ones we want in the particular
+    situation at hand -- they may be logically equivalent but have a
+    different syntactic form that fails to unify with the goal we are
+    trying to prove, or they actually may be logically weaker (for
+    preconditions) or stronger (for postconditions) than what we need. *)
+
+    For instance,
+
+      {(x == 3) [x := 3]} x := 3 {x == 3},
+
+    follows directly from the assignment rule, but
+
+      {true} x := 3 {x == 3}
+
+    does not.  This triple is valid, but it is not an instance of
+    [hoare_asgn] because true and (x == 3) [x := 3] are not
+    syntactically equal assertions.
+
+    However, they are logically _equivalent_, so if one triple is
+    valid, then the other must certainly be as well.  We can capture
+    this observation with the following rule:
+
+                {P'} s {Q}
+                  P <-> P'
+         -------------------------   (hoare_consequence_pre_equiv)
+                 {P} s {Q}
+*)
+
+(** Taking this line of thought a bit further, we can see that
+    strengthening the precondition or weakening the postcondition of a
+    valid triple always produces another valid triple. This
+    observation is captured by two _Rules of Consequence_.
+
+                {P'} c {Q}
+                  P -> P'
+         -----------------------------   (hoare_consequence_pre)
+                {P} s {Q}
+
+                {P} s {Q'}
+                 Q' -> Q
+         -----------------------------    (hoare_consequence_post)
+                {P} s {Q}
+*/
+
+/* ================================================================= */
+/** ** Conditionals 
+
+    What sort of rule do we want for reasoning about conditional
+    statements?
+
+    Certainly, if the same assertion Q holds after executing
+    either of the branches, then it holds after the whole conditional.
+    So we might be tempted to write:
+
+              {P} s1 {Q}
+              {P} s2 {Q}
+      ---------------------------------
+       {P} if b { s1 } else { s2 } {Q}
+
+    However, this is rather weak. For example, using this rule,
+    we cannot show
+   
+      { true }
+        if x == 0
+          { y := 2 }
+        else 
+          { y := x + 1 }
+      { x <= y }}
+   
+    since the rule tells us nothing about the state in which the
+    assignments take place in the "then" and "else" branches.
+
+    Fortunately, we can say something more precise.  In the
+    "then" branch, we know that the boolean expression b evaluates to
+    true, and in the "else" branch, we know it evaluates to false.
+    Making this information available in the premises of the rule gives
+    us more information to work with when reasoning about the behavior
+    of s1 and s2 (i.e., the reasons why they establish the
+    postcondition Q).
+
+                {P &&  b} s1 {Q}
+                {P && !b} s2 {Q}
+      -------------------------------------  (hoare_if)
+         {P} if b { s1 } else { s2 } {Q}
+*/
+
+/* ================================================================= */
+/** ** While Loops 
+
+/** The Hoare rule for while loops is based on the idea of an
+    _invariant_: an assertion whose truth is guaranteed before and
+    after executing a command.  An assertion [P] is an invariant of [c] if
+
+      {{P}} c {{P}}
+
+    holds.  Note that in the middle of executing [c], the invariant
+    might temporarily become false, but by the end of [c], it must be
+    restored. *)
+
+(**  As a first attempt at a [while] rule, we could try:
+
+             {{P}} c {{P}}
+      ---------------------------
+      {{P} while b do c end {{P}}
+
+    That rule is valid: if [P] is an invariant of [c], as the premise
+    requires, then no matter how many times the loop body executes,
+    [P] is going to be true when the loop finally finishes.
+
+    But the rule also omits two crucial pieces of information.  First,
+    the loop terminates when [b] becomes false.  So we can strengthen
+    the postcondition in the conclusion:
+
+              {{P}} c {{P}}
+      ---------------------------------
+      {{P} while b do c end {{P /\ ~b}}
+
+    Second, the loop body will be executed only if [b] is true.  So we
+    can also strengthen the precondition in the premise:
+
+            {{P /\ b}} c {{P}}
+      --------------------------------- (hoare_while)
+      {{P} while b do c end {{P /\ ~b}}
+*)
+
+(** That is the Hoare [while] rule.  Note how it combines
+    aspects of [skip] and conditionals:
+
+    - If the loop body executes zero times, the rule is like [skip] in
+      that the precondition survives to become (part of) the
+      postcondition.
+
+    - Like a conditional, we can assume guard [b] holds on entry to
+      the subcommand.
+*)
+
+
+
+
+/* ################################################################# */
+/** * Decorated Programs */
+
+/** The beauty of Hoare Logic is that it is _structure-guided_: the
+    structure of proofs exactly follows the structure of programs.
+
+    We can record the essential ideas of a Hoare-logic proof --
+    omitting low-level calculational details -- by "decorating" a
+    program with appropriate assertions on each of its commands.
+
+    Such a _decorated program_ carries within itself an argument for
+    its own correctness. 
+
+    For example, consider the program: 
+ */
+method LoopToZero_1(m : int, p : int) returns (x: int, z: int) {
+  x := m;
+  z := p;
+  while !(x == 0) {
+    z := z - 1;
+    x := x - 1;
+  }
+}
+
+/* 
+    Here is one possible specification for this program, in the
+    form of a Hoare triple:
+
+    { true }
+    x := m;
+    z := p;
+    while !(x == 0) {
+      z := z - 1;
+      x := x - 1;
+    }
+    { z == p - m }
+
+    and here is the equivalent specification in terms of 
+    Dafny's _requires_ and _ensures_ syntax:
+*/
+method LoopToZero_2(m : int, p : int) returns (x: int, z: int)
+  requires true
+  ensures z == p - m
+{
+  x := m;
+  z := p;
+  while !(x == 0) {
+    z := z - 1;
+    x := x - 1;
+  }
+}
+
+/** Here is a decorated version of this program, embodying a
+    proof of this specification:
+
+    { true } ->
+    { m == m }
+      x := m
+    { x == m } ->
+    { x == m && p == p };
+      z := p;
+    { x == m && z == p } ->
+    { z - x == p - m }
+      while !(x == 0) {
+        { z - x == p - m && ! (x == 0) } ->
+        { (z - 1) - (x - 1) == p - m }
+        z := z - 1
+        { z - (x - 1) == p - m };
+        x := x - 1
+        { z - x == p - m }
+      end
+    { z - x == p - m /\ !!(x == 0) } ->
+    { z == p - m }}
+*/
+
+/** That is, a decorated program consists of the program's text
+    interleaved with assertions (sometimes multiple assertions
+    separated by implications). 
+
+    A decorated program can be viewed as a compact representation of a
+    proof in Hoare Logic: the assertions surrounding each command
+    specify the Hoare triple to be proved for that part of the program
+    using one of the Hoare Logic rules, and the structure of the
+    program itself shows how to assemble all these individual steps
+    into a proof for the whole program. *)
+
+/** Dafny's goal is to verify such decorated programs "mostly
+    automatically."  But, before we can verify anything, we need to be
+    able to _find_ a proof for a given specification, and for this we
+    need to discover the right assertions. This can be done in an
+    almost mechanical way, with the exception of finding loop
+    invariants. We'll first explain in detail how to construct 
+    decorations for several short programs, all of which are 
+    loop-free or have simple loop invariants. We'll return
+    to finding more interesting loop invariants later. *)
+
+(* ================================================================= *)
+(** ** Example: Swapping *)
+
+(** Consider the following program, which swaps the values of two
+    variables using addition and subtraction (instead of by assigning
+    to a temporary variable).
+
+       x := x + y;
+       y := x - y;
+       x := x - y
+
+    We can give a proof, in the form of decorations, that this program is
+    correct -- i.e., it really swaps x and y -- as follows.
+
+    (1)    { x == m && y == n } ->
+    (2)    { (x + y) - ((x + y) - y) == n && (x + y) - y == m }
+             x := x + y;
+    (3)    { x - (x - y) == n && x - y == m }
+             y := x - y;
+    (4)    { x - y == n && y = m }
+             x := x - y
+    (5)    { x = n && y = m }
+
+    The decorations can be constructed as follows:
+
+      - We begin with the undecorated program (the unnumbered lines).
+
+      - We add the specification -- i.e., the outer precondition (1)
+        and postcondition (5). In the precondition, we use parameters
+        m and n to remember the initial values of variables x
+        and y so that we can refer to them in the postcondition (5).
+
+      - We work backwards, mechanically, starting from (5) and
+        proceeding until we get to (2). At each step, we obtain the
+        precondition of the assignment from its postcondition by
+        substituting the assigned variable with the right-hand-side of
+        the assignment. For instance, we obtain (4) by substituting
+        x with x - y in (5), and we obtain (3) by substituting y
+        with x - y in (4).
+
+    Finally, we verify that (1) logically implies (2) -- i.e., that
+    the step from (1) to (2) is a valid use of the law of
+    consequence -- by doing a bit of high-school algebra.
+*/
+
+(* ================================================================= *)
+(** ** Example: Simple Conditionals *)
+
+(** Here is a simple decorated program using conditionals:
+
+      (1)   { true }
+              if x <= y {
+      (2)      { true && x <= y } ->
+      (3)      { (y - x) + x == y || (y - x) + y == x }
+                 z := y - x
+      (4)      { z + x == y || z + y == x }
+              } else {
+      (5)       { true && ~(x <= y) } ->
+      (6)       { (x - y) + x == y || (x - y) + y = x }
+                z := x - y
+      (7)       { z + x = y || z + y = x }
+              }
+      (8)   { z + x = y || z + y = x }}
+
+These decorations can be constructed as follows:
+
+  - We start with the outer precondition (1) and postcondition (8).
+
+  - Following the format dictated by the [hoare_if] rule, we copy the
+    postcondition (8) to (4) and (7). We conjoin the precondition (1)
+    with the guard of the conditional to obtain (2). We conjoin (1)
+    with the negated guard of the conditional to obtain (5).
+
+  - In order to use the assignment rule and obtain (3), we substitute
+    [Z] by [Y - X] in (4). To obtain (6) we substitute [Z] by [X - Y]
+    in (7).
+
+  - Finally, we verify that (2) implies (3) and (5) implies (6). Both
+    of these implications crucially depend on the ordering of [X] and
+    [Y] obtained from the guard. For instance, knowing that [X <= Y]
+    ensures that subtracting [X] from [Y] and then adding back [X]
+    produces [Y], as required by the first disjunct of (3). Similarly,
+    knowing that [~ (X <= Y)] ensures that subtracting [Y] from [X]
+    and then adding back [Y] produces [X], as needed by the second
+    disjunct of (6). Note that [n - m + m = n] does _not_ hold for
+    arbitrary natural numbers [n] and [m] (for example, [3 - 5 + 5 =
+    5]). *)
+
+(** **** Exercise: 2 stars, standard, optional (if_minus_plus_reloaded)
+
+    N.b.: Although this exercise is marked optional, it is an
+    excellent warm-up for the (non-optional) [if_minus_plus_correct]
+    exercise below!
+
+    Fill in valid decorations for the following program: *)
+(*
+  {{ True }}
+    if X <= Y then
+              {{                         }} ->>
+              {{                         }}
+      Z := Y - X
+              {{                         }}
+    else
+              {{                         }} ->>
+              {{                         }}
+      Y := X + Z
+              {{                         }}
+    end
+  {{ Y = X + Z }}
+*)
+(**
+    Briefly justify each use of [->>].
+*)
+
+(** [] *)
+
+(* ================================================================= *)
+(** ** Example: Reduce to Zero *)
+
+(** Here is a [while] loop that is so simple that [True] suffices
+    as a loop invariant.
+
+        (1)    {{ True }}
+                 while X <> 0 do
+        (2)                  {{ True /\ X <> 0 }} ->>
+        (3)                  {{ True }}
+                   X := X - 1
+        (4)                  {{ True }}
+                 end
+        (5)    {{ True /\ ~(X <> 0) }} ->>
+        (6)    {{ X = 0 }}
+
+   The decorations can be constructed as follows:
+
+     - Start with the outer precondition (1) and postcondition (6).
+
+     - Following the format dictated by the [hoare_while] rule, we copy
+       (1) to (4). We conjoin (1) with the guard to obtain (2). We also
+       conjoin (1) with the negation of the guard to obtain (5).
+
+     - Because the final postcondition (6) does not syntactically match (5),
+       we add an implication between them.
+
+     - Using the assignment rule with assertion (4), we trivially substitute
+       and obtain assertion (3).
+
+     - We add the implication between (2) and (3).
+
+   Finally we check that the implications do hold; both are trivial. *)
+
+(* ================================================================= *)
+(** ** Example: Division *)
+
+(** Let's do one more example of simple reasoning about a loop.
+
+    The following Imp program calculates the integer quotient and
+    remainder of parameters [m] and [n].
+
+       X := m;
+       Y := 0;
+       while n <= X do
+         X := X - n;
+         Y := Y + 1
+       end;
+
+    If we replace [m] and [n] by concrete numbers and execute the program, it
+    will terminate with the variable [X] set to the remainder when [m]
+    is divided by [n] and [Y] set to the quotient. *)
+
+(** In order to give a specification to this program we need to
+    remember that dividing [m] by [n] produces a remainder [X] and a
+    quotient [Y] such that [n * Y + X = m /\ X < n].
+
+    It turns out that we get lucky with this program and don't have to
+    think very hard about the loop invariant: the invariant is just
+    the first conjunct, [n * Y + X = m], and we can use this to
+    decorate the program.
+
+      (1)  {{ True }} ->>
+      (2)  {{ n * 0 + m = m }}
+             X := m;
+      (3)                     {{ n * 0 + X = m }}
+             Y := 0;
+      (4)                     {{ n * Y + X = m }}
+             while n <= X do
+      (5)                     {{ n * Y + X = m /\ n <= X }} ->>
+      (6)                     {{ n * (Y + 1) + (X - n) = m }}
+               X := X - n;
+      (7)                     {{ n * (Y + 1) + X = m }}
+               Y := Y + 1
+      (8)                     {{ n * Y + X = m }}
+             end
+      (9)  {{ n * Y + X = m /\ ~ (n <= X) }} ->>
+     (10)  {{ n * Y + X = m /\ X < n }}
+
+    Assertions (4), (5), (8), and (9) are derived mechanically from
+    the invariant and the loop's guard.  Assertions (8), (7), and (6)
+    are derived using the assignment rule going backwards from (8)
+    to (6).  Assertions (4), (3), and (2) are again backwards
+    applications of the assignment rule.
+
+    Now that we've decorated the program it only remains to check that
+    the uses of the consequence rule are correct -- i.e., that (1)
+    implies (2), that (5) implies (6), and that (9) implies (10). This
+    is indeed the case:
+      - (1) ->> (2):  trivial, by algebra.
+      - (5) ->> (6):  because [n <= X], we are guaranteed that the
+        subtraction in (6) does not get zero-truncated.  We can
+        therefore rewrite (6) as [n * Y + n + X - n] and cancel the
+        [n]s, which results in the left conjunct of (5).
+      - (9) ->> (10):  if [~ (n <= X)] then [X < n].  That's straightforward
+        from high-school algebra.
+    So, we have a valid decorated program. *)
